Progress on composed action

src/Actions/ComposedAction.dfy
@@ -1,11 +1,10 @@
-
 include "Actions.dfy"
 
 module Composed {
 
   import opened Actions
 
-  class Compose<T, V(!new), R> extends Action<T, R> {
+  class Compose<T(!new), V(!new), R(!new)> extends Action<T, R> {
 
     const first: Action<T, V>
     const second: Action<V, R>
@@ -15,12 +14,15 @@ module Composed {
       ensures Valid() ==> this in Repr 
       ensures Valid() ==> 
         && CanProduce(consumed, produced)
-      decreases Repr, 0
+      decreases height, 0
     {
       && this in Repr
       && ValidComponent(first)
       && ValidComponent(second)
+      && first.Repr !! second.Repr
       && CanProduce(consumed, produced)
+      && forall ts, vs | first.CanProduce(ts, vs) :: 
+        exists rs :: second.CanProduce(vs, rs)
     }
 
     constructor(second: Action<V, R>, first: Action<T, V>) 
@@ -38,32 +40,41 @@ module Composed {
       consumed := [];
       produced := [];
       Repr := {this} + first.Repr + second.Repr;
+      height := first.height + second.height + 1;
     }
 
-    ghost predicate CanConsume(consumed: seq<T>, produced: seq<R>, next: T) {
+    ghost predicate CanConsume(consumed: seq<T>, produced: seq<R>, next: T)
+      decreases height
+    {
       exists vs: seq<V> :: 
         && first.CanProduce(consumed, vs)
         && first.CanConsume(consumed, vs, next)
     }
-    ghost predicate CanProduce(consumed: seq<T>, produced: seq<R>) {
-      exists vs: seq<V> :: first.CanProduce(consumed, vs) && second.CanProduce(vs, produced)
+    ghost predicate CanProduce(consumed: seq<T>, produced: seq<R>)
+      decreases height
+    {
+      exists vs: seq<V> :: 
+        && first.CanProduce(consumed, vs)
+        && second.CanProduce(vs, produced)
     }
 
     method Invoke(t: T) returns (r: R) 
       requires Valid()
       requires CanConsume(consumed, produced, t)
       modifies Repr
-      decreases Repr
+      decreases height
       ensures Valid()
-      ensures Repr <= old(Repr)
+      ensures fresh(Repr - old(Repr))
       ensures consumed == old(consumed) + [t]
       ensures produced == old(produced) + [r]
       ensures CanProduce(consumed, produced)
     {
       var v := first.Invoke(t);
+      
       r := second.Invoke(v);
 
       Update(t, r);
+      Repr := {this} + first.Repr + second.Repr;
     }
 
   }
